# Chapter 4: Equational Reasoning in Agda

This chapter looks to Graham Hutton's book _Programming in Haskell_ to use equational reasoning to prove properties of programing. Agda excels at this.
To start with, we define some 'helper' operators which allow proof in Agda to follow a logical set of steps, similar to those with pen and paper.
```
open import 03-curry-howard using (_‚â°_; refl; sym; trans)

begin_ : {A : Set} ‚Üí {x y : A} ‚Üí x ‚â° y ‚Üí x ‚â° y
begin p = p

_end : {A : Set} ‚Üí (x : A) ‚Üí x ‚â° x
x end = refl

_=‚ü®_‚ü©_ : {A : Set} ‚Üí (x : A) ‚Üí {y z : A}
       ‚Üí x ‚â° y ‚Üí y ‚â° z ‚Üí x ‚â° z
x =‚ü® p ‚ü© q = trans p q

_=‚ü®‚ü©_ : {A : Set} ‚Üí (x : A) ‚Üí {y : A} ‚Üí x ‚â° y ‚Üí x ‚â° y
x =‚ü®‚ü© q = x =‚ü® refl ‚ü© q

infix  1 begin_
infix  3 _end
infixr 2 _=‚ü®_‚ü©_
infixr 2 _=‚ü®‚ü©_
```

Let's try proving that `reverse`ing a singleton list does no change the list:
```
open import 01-intro-nat using (List; []; _‚à∑_; _++_)

[_] : {A : Set} ‚Üí A ‚Üí List A
[ x ] = x ‚à∑ []

reverse : {A : Set} ‚Üí List A ‚Üí List A
reverse [] = []
reverse (x ‚à∑ xs) = reverse xs ++ [ x ]

-- given the above definitions, let the proving begin - with the singleton case for now
reverse-singleton : {A : Set} (x : A) ‚Üí reverse [ x ] ‚â° [ x ]
reverse-singleton x =
  begin
    reverse [ x ]
  =‚ü®‚ü©
    reverse (x ‚à∑ [])
  =‚ü®‚ü©
    reverse [] ++ [ x ]
  =‚ü®‚ü©
    [] ++ [ x ]
  =‚ü®‚ü©
    [ x ]
  end
```

## Proof by cases and induction
Let's prove that, for all natural numbers `n`, `n + 0 = n` (noting that the definition of `_+_` defines `0 + n`, which has the operands flipped).
```
open import 01-intro-nat using (Nat; zero; succ; _+_)
open import 03-curry-howard using (cong)

add-n-zero : (n : Nat) ‚Üí n + zero ‚â° n
add-n-zero zero =     -- base (zero) case
  begin
    zero + zero       -- applying + (with `zero + m`;  m as zero)
  =‚ü®‚ü©
    zero
  end
add-n-zero (succ n) =
  begin
    (succ n) + zero   -- applying + (with `(succ n) + m`; m as zero)
  =‚ü®‚ü©
    succ (n + zero)
  =‚ü® cong succ (add-n-zero n)  ‚ü©  -- by induction
   succ n
  end
```

### Exercise 4.1. Prove that `m + succ n = succ (m + n)` for all `n, m ‚àà ‚Ñï`.
```
add-succ-n : (m n : Nat) ‚Üí m + (succ n) ‚â° succ (m + n)
add-succ-n zero n =
  begin
    zero + succ n
  =‚ü®‚ü©  -- apply `zero + m = m`
    succ n
  =‚ü®‚ü©
    succ (zero + n)
  end
add-succ-n (succ m) n =
  begin
    succ m + succ n
  =‚ü®‚ü©
    succ (m + succ n)
  =‚ü® cong succ (add-succ-n m n) ‚ü©
    succ (succ (m + n))
  end
```
<Continued>
Next, for use the previous lemma (`add-n-zero`) and the above one (`add-succ-n`) to prove commutativity of addition over ‚Ñï, i.e. that ‚àÄ m, n ‚àà ‚Ñï, `m + n = n + m`.
```
add-commute : (m n : Nat) ‚Üí m + n ‚â° n + m
add-commute m zero =
  begin  
    m + zero  -- case 1/2: `n` is zero
  =‚ü® add-n-zero m ‚ü©
    m
  =‚ü®‚ü©
    zero + m  -- we've swapped the order ‚áí it commutes
  end
add-commute m (succ n) =
  begin
    m + (succ n)  -- case 2/2: `n` is (succ n)  (*)
  =‚ü® (add-succ-n m n) ‚ü©
    succ (m + n)
  =‚ü® cong succ (add-commute m n) ‚ü©  -- by induction
    succ (n + m) 
  =‚ü®‚ü©
    (succ n) + m  -- we've swapped the order from (*) ‚áí it commutes and is shown by induction
  end
```

Continuing on from commutativity, let's prove that addition over ‚Ñï is associative, i.e. `l + (m + n) = (l + m) + n`:
```
add-assoc : (l m n : Nat) ‚Üí l + (m + n) ‚â° (l + m) + n
add-assoc zero m n =
  begin
     zero + (m + n)
   =‚ü®‚ü©
     m + n
   =‚ü®‚ü©
     (zero + m) + n
  end 
add-assoc (succ l) m n =
  begin
    (succ l) + (m + n)
  =‚ü®‚ü©
    succ (l + (m + n))
  =‚ü® cong succ (add-assoc l m n) ‚ü©
    succ ((l + m) + n)
  =‚ü®‚ü©
    (succ (l + m)) + n
  =‚ü®‚ü©
    (succ l + m) + n
  end
```

### Exercise 4.2. Consider the following function:
```
replicate : {A : Set} ‚Üí Nat ‚Üí A ‚Üí List A
replicate zero     _ = []
replicate (succ n) x = x ‚à∑ replicate n x
```
Prove that the length of `replicate n x` is always equal to n, by induction on the number n.
```
open import 01-intro-nat using (length)

replicate-is-length-n : {A : Set} ‚Üí (n : Nat) ‚Üí (x : A)
                      ‚Üí length (replicate n x) ‚â° n
replicate-is-length-n {A} zero x =
  begin
    length (replicate zero x)
  =‚ü®‚ü©
    length {A} []   -- note a type needs to be provided here, otherwise the type is ambiguous
  =‚ü®‚ü©
    zero
  end
replicate-is-length-n (succ n) x =
  begin
    length (replicate (succ n) x)
   =‚ü®‚ü©
    length (x ‚à∑ replicate n x)
   =‚ü®‚ü©
    succ (length (replicate n x))
   =‚ü® cong succ (replicate-is-length-n n x) ‚ü©
    succ n
  end
```

## Induction on lists
Now for something more insightful: proving that `reverse`ing a list twice yields the same list.
Towards this, we'll need to provide auxilliary lemmas, proving that  distributes over list concatenation (i.e. reversing a list comprised of two others is the same as reversing the two lists and 'flip' concatenating them), i.e.
`
  reverse (xs ++ ys) = reverse ys ++ reverse xs
`
(for this proof, and some subsequent proofs, the lemma showing associativity of the append function `_++_` will be needed, so is extracted here, rather than sitting in a `where`-clause)
```
append-assoc : {A : Set} ‚Üí (xs ys zs : List A)
                     ‚Üí (xs ++ ys) ++ zs ‚â° xs ++ (ys ++ zs)
append-assoc [] ys zs =
  begin
    ([] ++ ys) ++ zs
  =‚ü®‚ü©
    ys ++ zs
  =‚ü®‚ü©
    [] ++ (ys ++ zs)
  end
append-assoc (x ‚à∑ xs) ys zs =
  begin
    ((x ‚à∑ xs) ++ ys) ++ zs
  =‚ü®‚ü©
    (x ‚à∑ (xs ++ ys)) ++ zs
  =‚ü®‚ü©
    x ‚à∑ ((xs ++ ys) ++ zs)
  =‚ü® cong (x ‚à∑_) (append-assoc xs ys zs) ‚ü©
    x ‚à∑ (xs ++ (ys ++ zs))
  =‚ü®‚ü©
    (x ‚à∑ xs) ++ (ys ++ zs)
  end
```

```
reverse-reverse : {A : Set} ‚Üí (xs : List A) ‚Üí reverse (reverse xs) ‚â° xs
reverse-reverse [] =
  begin
    reverse (reverse [])
  =‚ü®‚ü©
    reverse []
  =‚ü®‚ü©
    []
   end
reverse-reverse (x ‚à∑ xs) = 
  begin
    reverse (reverse (x ‚à∑ xs))
  =‚ü®‚ü©
    reverse (reverse xs ++ [ x ])
  =‚ü® reverse-distributivity (reverse xs) [ x ] ‚ü©
    reverse [ x ] ++ reverse (reverse xs)
  =‚ü®‚ü©
   [ x ] ++ reverse (reverse xs)
  =‚ü® cong (x ‚à∑_) (reverse-reverse xs) ‚ü©  -- NOTE: (x ::_) is curried _‚à∑_ with the first argument applied, a.k.a 'section syntax`: `Œª xs ‚Üí x ‚à∑ xs`
    (x ‚à∑ xs)
  end
  where
    reverse-distributivity : {A : Set} ‚Üí (xs ys : List A)
                           ‚Üí reverse (xs ++ ys) ‚â° reverse ys ++ reverse xs
    reverse-distributivity [] ys =
      begin
        reverse ([] ++ ys)
      =‚ü®‚ü©
        reverse ys
      =‚ü® sym (append-[] (reverse ys)) ‚ü©
        reverse ys ++ []
      =‚ü®‚ü©
        reverse ys ++ reverse []
      end
      where
        append-[] : {A : Set} ‚Üí (xs : List A) ‚Üí xs ++ [] ‚â° xs
        append-[] [] =
          begin
            [] ++ []
          =‚ü®‚ü©
            []
          end
        append-[] (x ‚à∑ xs) =
          begin
            (x ‚à∑ xs) ++ []
          =‚ü®‚ü©
            x ‚à∑ (xs ++ [])
          =‚ü® cong (x ‚à∑_) (append-[] xs) ‚ü© 
            x ‚à∑ xs
          end
    reverse-distributivity (x ‚à∑ xs) ys =
      begin
        reverse ((x ‚à∑ xs) ++ ys)
      =‚ü®‚ü©
        reverse (x ‚à∑ (xs ++ ys))
      =‚ü®‚ü©
        reverse (xs ++ ys) ++ reverse [ x ]
      =‚ü®‚ü©
        reverse (xs ++ ys) ++ [ x ]
      =‚ü® cong (_++ [ x ]) (reverse-distributivity xs ys) ‚ü©
        (reverse ys ++ reverse xs) ++ [ x ]
      =‚ü® append-assoc (reverse ys) (reverse xs) [ x ] ‚ü©
        reverse ys ++ (reverse xs ++ [ x ]) 
      =‚ü®‚ü©
        reverse ys ++ reverse (x ‚à∑ xs)
      end
```
### Exercise 4.3. Proofs of `append-[]` and `append-assoc` above.


## Proving the functor laws for `map`.
The functor laws, for some functor `f`, comprise:
  Identity: `f id = id`
  Composition: `f (g ‚àò h) = f g ‚àò f g`

Let us prove these for `f` as `map` on `List`s.
```
open import 01-intro-nat using (id; map)

-- Identity Law
map-id : {A : Set} (xs : List A) ‚Üí map id xs ‚â° xs
map-id [] =
  begin
    map id []
  =‚ü®‚ü©
    []
  end
map-id (x ‚à∑ xs) =
  begin
    map id (x ‚à∑ xs)
  =‚ü®‚ü©
    id x ‚à∑ map id xs
  =‚ü®‚ü©
    x ‚à∑ map id xs
  =‚ü® cong (x ‚à∑_) (map-id xs) ‚ü©  -- by induction; using 'section syntax'
    x ‚à∑ xs
  end

-- Composition Law
_‚àò_ : {A B C : Set} ‚Üí (B ‚Üí C) ‚Üí (A ‚Üí B) ‚Üí (A ‚Üí C)
g ‚àò h = Œª x ‚Üí g (h x)

map-compose : {A B C : Set} ‚Üí (f : B ‚Üí C) (g : A ‚Üí B) (xs : List A)
            ‚Üí map (f ‚àò g) xs ‚â° map f (map g xs)
map-compose f g [] =
  begin
    map (f ‚àò g) []
  =‚ü®‚ü©
    []
  =‚ü®‚ü©
    map f []
  =‚ü®‚ü©
    map f (map g [])
  end
map-compose f g (x ‚à∑ xs) =
  begin
    map (f ‚àò g) (x ‚à∑ xs)
  =‚ü®‚ü©
    (f ‚àò g) x ‚à∑ map (f ‚àò g) xs
  =‚ü®‚ü©
    f (g x) ‚à∑ map (f ‚àò g) xs
  =‚ü® cong (f (g x) ‚à∑_) (map-compose f g xs) ‚ü©
    f (g x) ‚à∑ map f (map g xs)
  =‚ü®‚ü©
    map f (g x ‚à∑ map g xs)
  =‚ü®‚ü©
    map f (map g (x ‚à∑ xs))
  end
```

### Exercise 4.4. Prove that `length (map f xs) is equal to `length xs` for all `xs`.
```
map-length : {A B : Set} ‚Üí (f : A ‚Üí B) (xs : List A)
           ‚Üí length (map f xs) ‚â° length xs
map-length {A} f [] =
  begin
    length (map f [])
  =‚ü®‚ü©
    length {A} []
  end
map-length f (x ‚à∑ xs) =
   begin
     length (map f (x ‚à∑ xs))
   =‚ü®‚ü©
     length (f x ‚à∑ (map f xs))
   =‚ü®‚ü©
     succ (length (map f xs))
   =‚ü® cong succ (map-length f xs) ‚ü©
    succ (length xs)
   =‚ü®‚ü©
     length (x ‚à∑ xs)
   end
```

### Exercise 4.5 Define the functions `take` and `drop` that respectively return or re- move the first `n` elements of the list (or all elements if the list is shorter). Prove that for any number n and any list xs, we have `take n xs ++ drop n xs = xs`.
```
take : {A : Set} ‚Üí Nat ‚Üí List A ‚Üí List A
take zero     _        = []
{-# CATCHALL #-}
take _        []       = []
take (succ n) (x ‚à∑ xs) = x ‚à∑ take n xs

drop : {A : Set} ‚Üí Nat ‚Üí List A ‚Üí List A
drop zero     xs       = xs
drop (succ n) []       = []
drop (succ n) (x ‚à∑ xs) = drop n xs

take-drop : {A : Set} (n : Nat) (xs : List A)
         ‚Üí take n xs ++ drop n xs ‚â° xs
take-drop zero xs =
  begin
    take zero xs ++ drop zero xs
  =‚ü®‚ü©
    [] ++ xs
  =‚ü®‚ü©
    xs
  end
take-drop (succ n) [] =
  begin
    take (succ n) [] ++ drop (succ n) []
  =‚ü®‚ü©
    [] ++ []
  =‚ü®‚ü©
    []
  end
take-drop (succ n) (x ‚à∑ xs) =
  begin
    take (succ n) (x ‚à∑ xs) ++ drop (succ n) (x ‚à∑ xs)
  =‚ü®‚ü©
    (x ‚à∑ (take n xs)) ++ (drop n xs)
  =‚ü® cong (x ‚à∑_) (take-drop n xs) ‚ü©
    x ‚à∑ xs
  end
```

## Verifying Optimizations
It is widely known [TODO: link] that a na√Øve implementation of `reverse` using the plain concatenation function (`_++_` above) is inefficient since it needs to traverse the whole list, applying `_++_` each time. More efficient is to use a helper function with an accumulator storing the intermediate list, mid-reversal. In Agda, this can be achieved with:
```
-- helper function, which accumulates the results of reversing in `acc`
reverse-acc : {A : Set} ‚Üí List A ‚Üí List A ‚Üí List A
reverse-acc []       acc = acc
reverse-acc (x ‚à∑ xs) acc = reverse-acc xs (x ‚à∑ acc)

-- `reverse` but with the accumulator helper function
reverse‚Ä≤ : {A : Set} ‚Üí List A ‚Üí List A
reverse‚Ä≤ xs = reverse-acc xs []
```

Now, let us show that the implementation of `reverse‚Ä≤` is _equivalent_ to the original `reverse`.
There are two auxilliary lemmas needed here: `append-[]` and `append-assoc`. `append-assoc` has been extracted from a `where`-clause in `reverse-reverse` above; meanwhile, let's demonstrate the use of a `postulate` clause in Agda to supply `append-[]` to take this lemma as 'granted':
```
postulate
  append-[] : {A : Set} ‚Üí (xs : List A) ‚Üí xs ++ [] ‚â° xs
```

```
reverse‚Ä≤-reverse : {A : Set} ‚Üí (xs : List A) ‚Üí reverse‚Ä≤ xs ‚â° reverse xs
reverse‚Ä≤-reverse xs =
  begin
    reverse‚Ä≤ xs
  =‚ü®‚ü©
    reverse-acc xs []
  =‚ü® reverse-acc-lemma xs [] ‚ü©
    reverse xs ++ []
  =‚ü® append-[] (reverse xs) ‚ü©
    reverse xs
  end
  where
    reverse-acc-lemma : {A : Set} ‚Üí (xs ys : List A)
                      ‚Üí reverse-acc xs ys ‚â° reverse xs ++ ys
    reverse-acc-lemma [] ys =
      begin
        reverse-acc [] ys
      =‚ü®‚ü©
        ys
      =‚ü®‚ü©
        [] ++  ys
      =‚ü®‚ü©
        reverse [] ++ ys
      end
    reverse-acc-lemma (x ‚à∑ xs) ys =
      begin
        reverse-acc (x ‚à∑ xs) ys
      =‚ü®‚ü©
        reverse-acc xs (x ‚à∑ ys)
      =‚ü® reverse-acc-lemma xs (x ‚à∑ ys) ‚ü©  -- via induction
        reverse xs ++ (x ‚à∑ ys)
      =‚ü®‚ü©
        reverse xs ++ ([ x ] ++ ys)
      =‚ü® sym (append-assoc (reverse xs) [ x ] ys) ‚ü©
        (reverse xs ++ [ x ]) ++ ys
      =‚ü®‚ü©
        reverse (x ‚à∑ xs) ++ ys
      end
```

Following this proof on reversing lists, we can expand this to tree structures.
First, let us define a binary tree (Tree‚ÇÇ) in Agda:
```
data Tree‚ÇÇ (A : Set) : Set where
  leaf : A ‚Üí Tree‚ÇÇ A
  node : Tree‚ÇÇ A ‚Üí Tree‚ÇÇ A ‚Üí Tree‚ÇÇ A
```

Now, if we wish to flatten the tree to a list, we might use this more naiÃàve function:
```
flatten : {A : Set} ‚Üí Tree‚ÇÇ A ‚Üí List A
flatten (leaf l)     = [ l ]
flatten (node n‚ÇÅ n‚ÇÇ) = flatten n‚ÇÅ ++ flatten n‚ÇÇ
```
or, we may use a more efficient one with an accumulator (similar to `reverse‚Ä≤`)
```
flatten-acc : {A : Set} ‚Üí Tree‚ÇÇ A ‚Üí List A ‚Üí List A
flatten-acc (leaf l)     acc = l ‚à∑ acc 
flatten-acc (node n‚ÇÅ n‚ÇÇ) acc = flatten-acc n‚ÇÅ (flatten-acc n‚ÇÇ acc)

flatten‚Ä≤ : {A : Set} ‚Üí Tree‚ÇÇ A ‚Üí List A
flatten‚Ä≤ t = flatten-acc t []
```

Let's prove the two implementations above, `flatten` and `flatten‚Ä≤` are indeed equivalent.
First, we want to show that applying `flatten-acc` to `t xs` is equivalent to appending xs to `flatten t`:
```
flatten-acc-flatten : {A : Set} (t : Tree‚ÇÇ A) (xs : List A)
                    ‚Üí flatten-acc t xs ‚â° flatten t ++ xs
flatten-acc-flatten (leaf x) xs =
  begin
    flatten-acc (leaf x) xs
  =‚ü®‚ü©
    x ‚à∑ xs
  =‚ü®‚ü©
    [ x ] ++ xs
  =‚ü®‚ü©
    flatten (leaf x) ++ xs
  end
flatten-acc-flatten (node n‚ÇÅ n‚ÇÇ) xs =
  begin
    flatten-acc (node n‚ÇÅ n‚ÇÇ) xs
  =‚ü®‚ü©
    flatten-acc n‚ÇÅ (flatten-acc n‚ÇÇ xs)
  =‚ü® flatten-acc-flatten n‚ÇÅ (flatten-acc n‚ÇÇ xs) ‚ü©  -- induction on n‚ÇÅ
    flatten n‚ÇÅ ++ (flatten-acc n‚ÇÇ xs)
  =‚ü® cong (flatten n‚ÇÅ ++_) (flatten-acc-flatten n‚ÇÇ xs) ‚ü©
    flatten n‚ÇÅ ++ (flatten n‚ÇÇ ++ xs)
  =‚ü® sym (append-assoc (flatten n‚ÇÅ) (flatten n‚ÇÇ) xs) ‚ü©
    flatten (node n‚ÇÅ n‚ÇÇ) ++ xs
  end
```
Now we can continue to prove the equivalence of `flatten` and `flatten‚Ä≤`:
```
flatten‚Ä≤-flatten : {A : Set} ‚Üí (t : Tree‚ÇÇ A)
                 ‚Üí flatten‚Ä≤ t ‚â° flatten t
flatten‚Ä≤-flatten t =
  begin
    flatten‚Ä≤ t
  =‚ü®‚ü©
    flatten-acc t []
  =‚ü® flatten-acc-flatten t [] ‚ü©
    flatten t ++ []
  =‚ü® append-[] (flatten t) ‚ü©
    flatten t
  end
```
Exercise 4.6. `flatten‚Ä≤-flatten` completed above üéâ.





